working/composition/event_based_refinement/load_balancer/service_correspondence/multiplication_service/Composition.v.dfy
@@ -1,0 +1,79 @@
+include "MultiplicationServiceComponent.v.dfy"
+include "../addition_service/AdditionServiceSpec.t.dfy"
+include "../shared/AbstractNetwork.t.dfy"
+
+module ComposedNetwork refines AbstractNetwork {
+}
+
+module MultiplicationService {
+    import opened Types
+    import opened ComposedNetwork = Network
+    import MultSvc = MultiplicationServiceComponent
+    import AddSvc = AdditionServiceSpec
+
+    datatype Constants = Constants(
+        multSvc: MultSvc.Constants,
+        addSvc: AddSvc.Constants,
+        network: ComposedNetwork.Constants) 
+    {
+        ghost predicate WF() 
+        {
+            && multSvc.WF()
+            //&& addSvc.WF() // todo - should add well-formedness for spec
+            && multSvc.hosts[0].idSelf != addSvc.idSelf
+        }
+    }
+
+    datatype Variables = Variables(
+        multSvc: MultSvc.Variables,
+        addSvc: AddSvc.Variables,
+        network: ComposedNetwork.Variables) 
+    {
+        ghost predicate WF(c: Constants) {
+            && c.WF()
+            && multSvc.WF(c.multSvc)
+            //&& addSvc.WF(c.addSvc)
+        }
+    }
+
+    ghost predicate Init(c: Constants, v: Variables) {
+        && v.WF(c)
+        && MultSvc.Init(c.multSvc, v.multSvc)
+        && AddSvc.Init(c.addSvc, v.addSvc)
+        && ComposedNetwork.Init(c.network, v.network)
+    }
+
+    ghost predicate MultSvcAction(c: Constants, v: Variables, v': Variables, msgOps: MessageOps, hostId: ClientId)
+    {
+        && v.WF(c)
+        && v'.WF(c)
+        && MultSvc.Next(c.multSvc, v.multSvc, v'.multSvc, msgOps)
+        && v.addSvc == v'.addSvc
+        && ComposedNetwork.Next(c.network, v.network, v'.network, msgOps, hostId)
+        && hostId == c.multSvc.hosts[0].idSelf
+    }
+
+    ghost predicate AddSvcAction(c: Constants, v: Variables, v': Variables, msgOps: MessageOps, hostId: ClientId)
+    {
+        && v.WF(c)
+        && v'.WF(c)
+        && AddSvc.Next(c.addSvc, v.addSvc, v'.addSvc, msgOps)
+        && v.multSvc == v'.multSvc
+        && ComposedNetwork.Next(c.network, v.network, v'.network, msgOps, hostId)
+        && hostId == c.addSvc.idSelf
+    }
+
+    datatype Step =
+        | ComponentActionStep(hostId: ClientId)
+
+    ghost predicate NextStep(c: Constants, v: Variables, v': Variables, msgOps: MessageOps, step: Step)
+    {
+        || MultSvcAction(c, v, v', msgOps, step.hostId)
+        || AddSvcAction(c, v, v', msgOps, step.hostId)
+    }
+
+    ghost predicate Next(c: Constants, v: Variables, v': Variables, msgOps: MessageOps)
+    {
+        exists step :: NextStep(c, v, v', msgOps, step)
+    }
+}
