working/composition/event_based_refinement/load_balancer/service_correspondence/multiplication_service/RefinementProof.v.dfy
@@ -1,0 +1,89 @@
+include "RefinementObligation.t.dfy"
+
+module RefinementProof refines RefinementTheorem {
+    ghost function ConstantsAbstraction(c: Constants) : Spec.Constants
+        //requires c.WF()
+    {
+        Spec.Constants
+    }
+
+    ghost function VariablesAbstraction(c: Constants, v: Variables) : Spec.Variables
+        //requires v.WF(c)
+    {
+        Spec.Variables(v.multSvc.hosts[0].requests, v.multSvc.hosts[0].replies)
+    }
+
+    // todo -- generalize these invariants and bake them into the system model?
+    ghost predicate Inv_AddSvcCorrespondence(c: Constants, v: Variables)
+        requires v.WF(c)
+    {
+        && (forall pkt: Message<seq<byte>> :: 
+            && pkt in v.network.sentMsgs
+            && AddSvc.ParseServiceReply(pkt.msg).Some? ==>
+                exists request: Message<AddSvc.ServiceRequest> :: 
+                && Message(pkt.src, pkt.dest, AddSvc.ParseServiceReply(pkt.msg).value) in v.addSvc.replies
+                && request in v.addSvc.requests 
+                && request.src == pkt.dest
+                && request.dest == pkt.src)
+        && (forall request: Message<AddSvc.ServiceRequest> ::
+            && request in v.addSvc.requests ==>
+            && Message(request.src, request.dest, AddSvc.MarshallServiceRequest(request.msg)) in v.network.sentMsgs)
+    }
+
+    ghost predicate Inv_MultSvcCorrespondence(c: Constants, v: Variables)
+        requires v.WF(c)
+    {
+        && (forall pkt: Message<seq<byte>> :: 
+            && pkt in v.network.sentMsgs
+            && Spec.ParseServiceReply(pkt.msg).Some? ==>
+                exists request: Message<Spec.ServiceRequest> :: 
+                && Message(pkt.src, pkt.dest, Spec.ParseServiceReply(pkt.msg).value) in v.multSvc.hosts[0].replies
+                && request in v.multSvc.hosts[0].requests 
+                && request.src == pkt.dest
+                && request.dest == pkt.src)
+        && (forall request: Message<Spec.ServiceRequest> ::
+            && request in v.multSvc.hosts[0].requests ==>
+            && Message(request.src, request.dest, Spec.MarshallServiceRequest(request.msg)) in v.network.sentMsgs)
+    }
+
+    ghost predicate Inv_AddSvcImpl(c: Constants, v: Variables)
+        requires v.WF(c)
+    {
+        && (forall pkt: Message<seq<byte>> :: 
+            && pkt in v.network.sentMsgs
+            && AddSvc.ParseServiceReply(pkt.msg).Some? ==>
+                exists request: Message<AddSvc.ServiceRequest> :: 
+                && request in v.addSvc.requests 
+                && AddSvc.ParseServiceReply(pkt.msg).value == AddSvc.AddReply(request.msg.seqNo, request.msg.x + request.msg.y))
+    }
+
+    ghost predicate Inv(c: Constants, v: Variables)
+    {
+        && v.WF(c)
+        && Inv_AddSvcCorrespondence(c, v)
+        && Inv_MultSvcCorrespondence(c, v)
+    }
+
+    lemma RefinementInit(c: Constants, v: Variables)
+        // requires Init(c, v)
+        // ensures Inv(c, v)
+        // ensures Spec.Init(ConstantsAbstraction(c), VariablesAbstraction(c, v))
+    {}
+    
+    lemma RefinementNext(c: Constants, v: Variables, v': Variables, msgOps: MessageOps)
+        // requires Next(c, v, v', msgOps)
+        // requires Inv(c, v)
+        // ensures Inv(c, v') 
+        // ensures 
+        //     || Spec.Next(ConstantsAbstraction(c), VariablesAbstraction(c, v), VariablesAbstraction(c, v'), MessageOps(ServiceRequestsAbstraction(msgOps.recv), ServiceRepliesAbstraction(msgOps.send)))
+        //     || (VariablesAbstraction(c, v) == VariablesAbstraction(c, v') && ServiceRequestsAbstraction(msgOps.recv) == {} && ServiceRepliesAbstraction(msgOps.send) == {})
+    {
+        if (Spec.Next(ConstantsAbstraction(c), VariablesAbstraction(c, v), VariablesAbstraction(c, v'), MessageOps(ServiceRequestsAbstraction(msgOps.recv), ServiceRepliesAbstraction(msgOps.send)))) {
+
+        }
+        else {
+            assume false;
+        }
+    }
+
+}
